Updated Curve25519_Procedures with latest proof

proof/crypto_scalarmult/curve25519/amd64/common/Curve25519_Procedures.ec
@@ -1,10 +1,10 @@
-require import Bool List Int IntExtra IntDiv CoreMap Real Zp.
-from Jasmin require import JModel.
+require import Bool List Int IntDiv CoreMap Real Zp_25519 Ring Distr StdOrder BitEncoding Zp_25519 W64limbs.
+from Jasmin require import JModel JWord JModel_x86.
 require import Curve25519_Spec.
-require import Curve25519_Hop1.
-import Zp ZModpRing Curve25519_Spec Curve25519_Hop1.
+require import Curve25519_Operations.
+import Zp Ring.IntID StdOrder.IntOrder BitEncoding.BS2Int.
 
-module MHop2 = {
+module CurveProcedures = {
 
   (* h = f + g *)
   proc add(f g : zp) : zp = 
@@ -50,71 +50,123 @@ module MHop2 = {
   (* iterated sqr *)
   proc it_sqr (i : int, f : zp) : zp =
   {
-    var h : zp;
-    h <- witness;
+    var h, g: zp;
+    var ii, counter: int;
 
+    counter <- 1;
+    g <- f;
+    ii <- i;
     h <@ sqr(f);
-    i <- i - 1;
-    f <@ sqr(h);
-    i <- i - 1;
 
-    while (0 < i) {
-      h <@ sqr(f);
-      i <- i - 1;
-      f <@ sqr(h);
-      i <- i - 1;
+    ii <- ii - 1;
+    while (0 < ii) {
+      h <@ sqr(h);
+      counter <- counter + 1;
+      ii <- ii - 1;
     }
+  return h;
+}
 
+proc it_sqr_aux (a : zp, l : int) : zp = {
+  var f, h: zp;
+  var ii: int;
+  ii <- l;
+  h <@ sqr(a);
+  f <@ sqr(h);
+  ii <- ii - 1;
+  while (0 < ii) {
+   h <@ sqr(f);
+   f <@ sqr(h);
+   ii <- ii - 1;
+}
     return f;
   }
 
   (* f ** 2**255-19-2 *)
-  proc invert (z1' : zp) : zp =
+  proc invert (fs : zp) : zp =
   {
-    var t0 : zp;
-    var t1 : zp;
-    var t2 : zp;
-    var t3 : zp;
+    var t1s : zp;
+    var t0s : zp;
+    var t2s : zp;
+    var t3s : zp;
 
-    t0 <- witness;
-    t1 <- witness;
-    t2 <- witness;
-    t3 <- witness;
+    t0s <- witness;
+    t1s <- witness;
+    t2s <- witness;
+    t3s <- witness;
 
-    t0 <@ sqr (z1');
-    t1 <@ sqr (t0);
-    t1 <@ sqr (t1);
-    t1 <@ mul (z1', t1);
-    t0 <@ mul (t0,  t1);
-    t2 <@ sqr (t0);
-    t1 <@ mul (t1, t2);
-    t2 <@ sqr (t1);
-    t2 <@ it_sqr (4, t2);
-    t1 <@ mul (t1, t2);
-    t2 <@ it_sqr (10, t1);
-    t2 <@ mul (t1, t2);
-    t3 <@ it_sqr (20, t2);
-    t2 <@ mul (t2, t3);
-    t2 <@ it_sqr (10, t2);
-    t1 <@ mul (t1, t2);
-    t2 <@ it_sqr (50, t1);
-    t2 <@ mul (t1, t2);
-    t3 <@ it_sqr (100, t2);
-    t2 <@ mul (t2, t3);
-    t2 <@ it_sqr (50, t2);
-    t1 <@ mul (t1, t2);
-    t1 <@ it_sqr (4, t1);
-    t1 <@ sqr (t1);
-    t1 <@ mul (t0, t1);
-    return t1;
+    t0s <@ sqr (fs);
+    t1s <@ sqr (t0s);
+    t1s <@ sqr (t1s);
+    t1s <@ mul (fs, t1s);
+    t0s <@ mul (t0s, t1s);
+    t2s <@ sqr (t0s);
+    t1s <@ mul (t1s, t2s);
+    t2s <@ sqr (t1s);
+    t2s <@ it_sqr (t2s,4);
+    t1s <@ mul (t1s, t2s);
+    t2s <@ it_sqr (t1s,10);
+    t2s <@ mul (t1s, t2s);
+    t3s <@ it_sqr (t2s,20);
+    t2s <@ mul(t2s, t3s);
+    t2s <@ it_sqr (t2s,10);
+    t1s <@ mul (t1s, t2s);
+    t2s <@ it_sqr (t1s,50);
+    t2s <@ mul (t1s, t2s);
+    t3s <@ it_sqr (t2s,100);
+    t2s <@ mul (t2s, t3s);
+    t2s <@ it_sqr (t2s,50);
+    t1s <@ mul (t1s, t2s);
+    t1s <@ it_sqr (t1s,4);
+    t1s <@ sqr (t1s);
+    t1s <@ mul (t0s, t1s);
+    return t1s;
   }
   
+proc invert_helper (fs : zp) : zp =
+{
+    var t1s : zp;
+    var t0s : zp;
+    var t2s : zp;
+    var t3s : zp;
+    t0s <- witness;
+    t1s <- witness;
+    t2s <- witness;
+    t3s <- witness;
+    t0s <@ sqr (fs);
+    t1s <@ sqr (t0s);
+    t1s <@ sqr (t1s);
+    t1s <@ mul (t1s, fs);
+    t0s <@ mul (t0s, t1s);
+    t2s <@ sqr (t0s);
+    t1s <@ mul (t1s, t2s);
+    t2s <@ sqr (t1s);
+    t2s <@ it_sqr (t2s, 4);
+    t1s <@ mul (t1s, t2s);
+    t2s <@ it_sqr (t1s, 10);
+    t2s <@ mul (t2s, t1s);
+    t3s <@ it_sqr (t2s, 20);
+    t2s <@ mul(t2s, t3s);
+    t2s <@ it_sqr (t2s, 10);
+    t1s <@ mul (t1s, t2s);
+    t2s <@ it_sqr (t1s, 50);
+    t2s <@ mul (t2s, t1s);
+    t3s <@ it_sqr (t2s, 100);
+    t2s <@ mul (t2s, t3s);
+    t2s <@ it_sqr (t2s, 50);
+    t1s <@ mul (t1s, t2s);
+    t1s <@ it_sqr (t1s, 4);
+    t1s <@ sqr (t1s);
+    t1s <@ mul (t1s, t0s);
+    return t1s;
+}
+
   proc cswap (x2 z2 x3 z3 : zp, toswap : bool) : zp * zp * zp * zp =
   {
-    if(toswap)
-    { (x2,z2,x3,z3) = (x3,z3,x2,z2); }
-    else
-    { (x2,z2,x3,z3) = (x2,z2,x3,z3); }
+    if(toswap){
+     (x2,z2,x3,z3) <- (x3,z3,x2,z2);
+    }else{
+     (x2,z2,x3,z3) <- (x2,z2,x3,z3);}
     return (x2,z2,x3,z3);
   }
 
@@ -123,7 +175,7 @@ module MHop2 = {
     return k'.[ctr];
   }
 
-  proc decode_scalar_25519 (k' : W256.t) : W256.t =
+  proc decode_scalar (k' : W256.t) : W256.t =
   {
     k'.[0] <- false;
     k'.[1] <- false;
@@ -161,6 +213,13 @@ module MHop2 = {
     return (x2, z2, x3, z3);
   }
   
+proc decode_u_coordinate_base () : zp =
+  {
+      var u' : zp;
+      u' <@ decode_u_coordinate (W256.of_int 9);
+      return u';
+ }
+
   proc add_and_double (init x2 z2 x3 z3 : zp) : zp * zp * zp * zp =
   {
     var t0 : zp;
@@ -170,7 +229,7 @@ module MHop2 = {
     t1 <- witness;
     t2 <- witness;
     t0 <@ sub (x2, z2);
-    x2 <@ add (x2, z2);
+    x2 <@ add (z2, x2);
     t1 <@ sub (x3, z3);
     z2 <@ add (x3, z3);
     z3 <@ mul (x2, t1);
@@ -190,11 +249,11 @@ module MHop2 = {
     return (x2, z2, x3, z3);
   }
 
-  proc montgomery_ladder_step (k' : W256.t, 
-                               init' x2 z2 x3 z3 : zp,
-                               swapped : bool,
+  proc montgomery_ladder_step (k' : W256.t
+                               init' x2 z2 x3 z3 : zp
+                               swapped : bool
                                ctr' : int) : zp * zp * zp * zp * bool =
-  { 
+  {
     var bit : bool;
     var toswap : bool;
     bit <@ ith_bit (k', ctr');
@@ -206,7 +265,7 @@ module MHop2 = {
     return (x2, z2, x3, z3, swapped);
   }
 
-  proc montgomery_ladder (init' : zp, k' : W256.t) : zp * zp * zp * zp = 
+  proc montgomery_ladder (init' : zp, k' : W256.t) : zp * zp * zp * zp =
   {
     var x2 : zp;
     var z2 : zp;
@@ -221,7 +280,7 @@ module MHop2 = {
     (x2, z2, x3, z3) <@ init_points (init');
     ctr <- 254;
     swapped <- false;
-    while (0 <= ctr)
+    while (0 < ctr)
     { (x2, z2, x3, z3, swapped) <@
         montgomery_ladder_step (k', init', x2, z2, x3, z3, swapped, ctr);
       ctr <- ctr - 1;
@@ -238,58 +297,93 @@ module MHop2 = {
     (* no need to 'freeze' or 'tobytes' r in this spec *)
     return (W256.of_int (asint r));
   }
+proc scalarmult_internal(u'': zp,  k': W256.t ) : W256.t =   {
+  var x2 : zp;
+  var z2 : zp;
+  var x3 : zp;
+  var z3 : zp;
+  var r : W256.t;
+  r <- witness;
+  x2 <- witness;
+  x3 <- witness;
+  z2 <- witness;
+  z3 <- witness;
+  (x2, z2, x3, z3) <@ montgomery_ladder(u'', k');
+  r <@ encode_point(x2, z2);
+  return r;
+}
 
   proc scalarmult (k' u' : W256.t) : W256.t =
   {
     var u'' : zp;
-    var x2 : zp;
-    var z2 : zp;
-    var x3 : zp;
-    var z3 : zp;
     var r : W256.t;
-   
     r <- witness;
-    x2 <- witness;
-    x3 <- witness;
-    z2 <- witness;
-    z3 <- witness;
 
-    k'  <@ decode_scalar_25519 (k');
+    k'  <@ decode_scalar (k');
     u'' <@ decode_u_coordinate (u');
-    (x2, z2, x3, z3) <@ montgomery_ladder (u'', k');
-    r <@ encode_point (x2, z2);
+    r   <@ scalarmult_internal(u'', k');
     return r;
   }
+
+proc scalarmult_base(k': W256.t) : W256.t =  {
+  var u'' : zp;
+  var x2 : zp;
+  var z2 : zp;
+  var x3 : zp;
+  var z3 : zp;
+  var r : W256.t;
+  r <- witness;
+  x2 <- witness;
+  x3 <- witness;
+  z2 <- witness;
+  z3 <- witness;
+  k'  <@ decode_scalar (k');
+u'' <@ decode_u_coordinate_base ();
+  r   <@ scalarmult_internal(u'', k');
+
+  return r; }
 }.
 
 (** step 1 : decode_scalar_25519 **)
-lemma eq_h2_decode_scalar_25519 k:
-  hoare [ MHop2.decode_scalar_25519 : k' = k
-          ==> res = decodeScalar25519 k].
+lemma eq_proc_op_decode_scalar k:
+  hoare [ CurveProcedures.decode_scalar: k' = k
+          ==> res = spec_decode_scalar_25519 k].
 proof.
-  proc; wp; rewrite /decodeScalar25519 /=; skip.
+  proc; wp; rewrite /spec_decode_scalar_25519 /=; skip.
   move => _ hk; rewrite hk //.
 qed.
 
 (** step 2 : decode_u_coordinate **)
-lemma eq_h2_decode_u_coordinate u:
-  hoare [ MHop2.decode_u_coordinate : u' = u
-          ==> res = decodeUCoordinate u].
+lemma eq_proc_op_decode_u_coordinate u:
+  hoare [ CurveProcedures.decode_u_coordinate : u' = u
+          ==> res = inzp (to_uint (spec_decode_u_coordinate u))].
 proof.
-  proc; wp; rewrite /decode_u_coordinate /=; skip.
+  proc; wp. rewrite /spec_decode_u_coordinate /=; skip.
   move => _ hu; rewrite hu //.
 qed.
 
-(** step 3 : ith_bit **)
-lemma eq_h2_ith_bit (k : W256.t) i:
-  hoare [MHop2.ith_bit : k' = k /\ ctr = i ==> res = ith_bit k i].
+lemma eq_proc_op_decode_u_coordinate_base:
+  hoare[ CurveProcedures.decode_u_coordinate_base:
+      true
+      ==>
+      res = inzp (to_uint (spec_decode_u_coordinate( W256.of_int 9)))
+  ].
 proof.
-  proc. rewrite /ith_bit. skip => />.
+  proc *; inline 1; wp.
+  ecall (eq_proc_op_decode_u_coordinate (W256.of_int 9)).
+  auto => />.
+ qed.
+
+(** step 3 : ith_bit **)
+lemma eq_proc_op_ith_bit (k : W256.t) i:
+  hoare [CurveProcedures.ith_bit : k' = k /\ ctr = i ==> res = spec_ith_bit k i].
+proof.
+  proc. rewrite /spec_ith_bit. skip => />.
 qed.
 
 (** step 4 : cswap **)
-lemma eq_h2_cswap (t : (zp * zp) * (zp * zp) )  b:
-  hoare [MHop2.cswap : x2 = (t.`1).`1 /\
+lemma eq_proc_op_cswap (t : (zp * zp) * (zp * zp) )  b:
+  hoare [CurveProcedures.cswap : x2 = (t.`1).`1 /\
                        z2 = (t.`1).`2 /\
                        x3 = (t.`2).`1 /\
                        z3 = (t.`2).`2 /\
@@ -300,24 +394,24 @@ proof.
 qed.
 
 (** step 5 : add_and_double **)
-lemma eq_h2_add_and_double (qx : zp) (nqs : (zp * zp) * (zp * zp)):
-  hoare [MHop2.add_and_double : init = qx /\ 
+lemma eq_proc_op_add_and_double (qx : zp) (nqs : (zp * zp) * (zp * zp)):
+  hoare [CurveProcedures.add_and_double : init = qx /\ 
                                 x2 = nqs.`1.`1 /\
                                 z2 = nqs.`1.`2 /\
                                 x3 = nqs.`2.`1 /\
                                 z3 = nqs.`2.`2
-         ==> ((res.`1, res.`2),(res.`3, res.`4)) = add_and_double1 qx nqs].
+         ==> ((res.`1, res.`2),(res.`3, res.`4)) = op_add_and_double qx nqs].
 proof.
   proc; inline *; wp; skip.
-  rewrite /add_and_double1 /=. smt(expr2).
+  rewrite /op_add_and_double /=. rewrite !ZModpRing.expr2. smt().
 qed.
 
 (** step 6 : montgomery_ladder_step **)
-lemma eq_h2_montgomery_ladder_step (k : W256.t) 
+lemma eq_proc_op_montgomery_ladder_step (k : W256.t) 
                                    (init : zp)
                                    (nqs : (zp * zp) * (zp * zp) * bool) 
                                    (ctr : int) :
-  hoare [MHop2.montgomery_ladder_step : k' = k /\ 
+  hoare [CurveProcedures.montgomery_ladder_step : k' = k /\
                                         init' = init /\
                                         x2 = nqs.`1.`1 /\
                                         z2 = nqs.`1.`2 /\
@@ -326,163 +420,205 @@ lemma eq_h2_montgomery_ladder_step (k : W256.t)
                                         swapped = nqs.`3 /\
                                         ctr' = ctr
          ==> ((res.`1, res.`2),(res.`3, res.`4),res.`5) =
-             montgomery_ladder3_step k init nqs ctr].
+             op_montgomery_ladder3_step k init nqs ctr].
 proof.
   proc => /=.
-  ecall (eq_h2_add_and_double init (cswap (select_tuple_12 nqs) (nqs.`3 ^^ (ith_bit k ctr)))).
+  ecall (eq_proc_op_add_and_double init (cswap (select_double_from_triple nqs) (nqs.`3 ^^ (spec_ith_bit k ctr)))).
   wp.
-  ecall (eq_h2_cswap (select_tuple_12 nqs) (nqs.`3 ^^ (ith_bit k ctr))).
+  ecall (eq_proc_op_cswap (select_double_from_triple nqs) (nqs.`3 ^^ (spec_ith_bit k ctr))).
   wp.
-  ecall (eq_h2_ith_bit k ctr). auto.
-  rewrite /montgomery_ladder3_step => /#.
+  ecall (eq_proc_op_ith_bit k ctr). auto.
+  rewrite /op_montgomery_ladder3_step => /#.
 qed.
 
 (** step 7 : montgomery_ladder **)
 lemma unroll_ml3s  k init nqs (ctr : int) : (** unroll montgomery ladder 3 step **)
   0 <= ctr =>
-    foldl (montgomery_ladder3_step k init)
+    foldl (op_montgomery_ladder3_step k init)
           nqs
           (rev (iota_ 0 (ctr+1)))
     =
-    foldl (montgomery_ladder3_step k init)
-          (montgomery_ladder3_step k init nqs ctr)
+    foldl (op_montgomery_ladder3_step k init)
+          (op_montgomery_ladder3_step k init nqs ctr)
           (rev (iota_ 0 (ctr))).
 proof.
 move => ctrge0.
 rewrite 2!foldl_rev iotaSr //= -cats1 foldr_cat => /#.
 qed.
 
-lemma eq_h2_montgomery_ladder (init : zp)
+lemma eq_proc_op_montgomery_ladder (init : zp)
                               (k : W256.t) :
-  hoare [MHop2.montgomery_ladder : init' = init /\
+  hoare [CurveProcedures.montgomery_ladder : init' = init /\
                                    k.[0] = false /\
                                    k' = k
          ==> ((res.`1, res.`2),(res.`3,res.`4)) =
-             select_tuple_12 (montgomery_ladder3 init k)].
+             select_double_from_triple (op_montgomery_ladder3 init k)].
 proof.
 proc.
-  inline MHop2.init_points. sp. simplify.
-  rewrite /montgomery_ladder3.
+  inline CurveProcedures.init_points. sp. simplify.
+  rewrite /op_montgomery_ladder3.
 
-  while (foldl (montgomery_ladder3_step k' init')
+  while (foldl (op_montgomery_ladder3_step k' init')
                ((Zp.one, Zp.zero), (init, Zp.one), false)
                (rev (iota_ 0 255))
          =
-         foldl (montgomery_ladder3_step k' init')
+         foldl (op_montgomery_ladder3_step k' init')
                ((x2,z2), (x3,z3), swapped)
-               (rev (iota_ 0 (ctr+1)))
+               (rev (iota_ 0 (ctr)))
          ).
-  wp.
-  ecall (eq_h2_montgomery_ladder_step k' init' ((x2,z2),(x3,z3),swapped) ctr).
+  wp. sp.
+  ecall (eq_proc_op_montgomery_ladder_step k' init' ((x2,z2),(x3,z3),swapped) ctr).
   skip. simplify.
   move => &hr [?] ? ? ?. smt(unroll_ml3s).
   skip. move => &hr [?] [?] [?] [?] [?] [?] [?] [?] [?] [?] [?] [?] [?] ?. subst.
   split; first by done.
-  move => ? ? ? ? ? ? ?.
-  have _ : rev (iota_ 0 (ctr0 + 1)) = []; smt(iota0).
+  move => H ? ? ? ? ? ? ?.
+  have _ : rev (iota_ 0 (H)) = []; smt(iota0).
 qed.
 
 (** step 8 : iterated square **)
-lemma it_sqr1_m2_exp4 (e : int) (z : zp) :
-  0 <= e - 2 => it_sqr1 e z = it_sqr1 (e-2) (exp (exp z 2) 2).
-proof.
-  rewrite expE // /= => ?.
-  rewrite !eq_it_sqr1. smt(). trivial.
-  rewrite /it_sqr (*expE*).
-  (* directly rewriting expE takes too long *)
-  have ee :  exp (exp z 4) (2 ^ (e - 2)) =  exp z (2^2 * 2 ^ (e - 2)). smt(expE).
-  rewrite ee. congr.
-  rewrite pow_add //.
-qed.
 
-lemma it_sqr1_0 (e : int) (z : zp) :
-  0 = e => it_sqr1 e z = z.
-proof.
-  move => ?.
-  rewrite eq_it_sqr1. smt().
-  rewrite /it_sqr. subst. simplify.
-  rewrite expr1 //.
-qed.
 
-lemma eq_h2_it_sqr (e : int) (z : zp) : 
-  hoare[MHop2.it_sqr :
-         i = e && 2 <= i && i %% 2 = 0 && f =  z 
+lemma eq_proc_op_it_sqr (e : int) (z : zp) :
+  hoare[CurveProcedures.it_sqr : 
+         i = e && 1 <= i && f =  z 
          ==>
-        res = it_sqr1 e z].
+        res = op_it_sqr1 e z].
 proof.
-  proc. inline MHop2.sqr. simplify.
-  while ( 0 <= i && i %% 2 = 0 && it_sqr1 e z = it_sqr1 i f).
-  wp. skip.
-
-  (** alternative version with progress **)
-  (*
-            progress. smt(). smt(). smt(it_sqr1_m2_exp4).
-  wp. skip. progress. smt(). smt(). smt(it_sqr1_m2_exp4).
-  smt(it_sqr1_0).
-  *)
-
-  move => &hr [[?]] [?] hin ?. simplify.
-  split; first by smt(). move => ?.
-  split; first by smt(). move => ?.
-  rewrite hin. move : H2. apply it_sqr1_m2_exp4.
-  wp. skip.
-  move => &hr [?] [?] [?] ?. simplify.
-  split.
-  split; first by smt(). move => ?.
-  split; first by smt(). move => ?.
-  subst. move : H3.  apply it_sqr1_m2_exp4.
-  move => ? ? ? [?] [?] ->. subst.
-  have ieq0 : i0 = 0. smt().
-  rewrite it_sqr1_0 /#.
+  proc. inline CurveProcedures.sqr. sp. wp.  simplify.
+  while (0 <= i && 0 <= ii && op_it_sqr1 e z = op_it_sqr1 ii h).
+  wp; skip.
+  move => &hr [[H [H0 H1 H2 H3]]]. split.
+  apply H. move => H4. split. rewrite /H3.
+  smt(). move => H5. rewrite /H3.
+  smt(op_it_sqr1_m2_exp1). skip.
+  move => &hr [H [H0 [H1 [H2 [H3]]]]] H4. split. split. smt(). move => H5. split. smt(). move => H6.
+  smt(op_it_sqr1_m2_exp1). move => H5 H6 H7 [H8 [H9 H10]]. smt(op_it_sqr1_0).
 qed.
+
+lemma eq_proc_op_it_sqr_x2 (e : int) (z : zp) :
+  hoare[CurveProcedures.it_sqr :
+    i%/2 = e && 2 <= i && i %% 2 = 0 && f = z
+    ==>
+    res = op_it_sqr1_x2 e z].
+proof.
+  proc. inline CurveProcedures.sqr. sp. wp. simplify.
+  while (0 <= i && 0 <= ii && 2*e = i && op_it_sqr1_x2 e z = op_it_sqr1 i f && op_it_sqr1 (2*e) z = op_it_sqr1 ii h).
+  wp; skip. 
+  move => &hr [[H]] [H0] [H1] [H2] H3 H4 H5.
+  split. assumption. move => H6.
+  split. smt(). move => H7.
+  split. assumption. move => H8.
+  split. assumption. move => H9.
+  rewrite H3 /H5 => />. smt(op_it_sqr1_m2_exp1). skip.
+move => &hr [H] [H0] [H1] [H2] [H3] [H4] [H5] [H6] H7.
+  do! split.
+  + smt(). move => H8.
+  split. rewrite H3; first smt(). move => H9.
+  split. rewrite -H4. auto => />. smt(). move => H10.
+  split. rewrite eq_op_it_sqr1_x2. rewrite -H4. smt().
+  rewrite eq_op_it_sqr1. smt().
+  rewrite /op_it_sqr_x2 /op_it_sqr H7 -H10. congr.
+  rewrite exprM => />. move => H11.
+  rewrite !eq_op_it_sqr1; first smt(). smt().
+  rewrite !/op_it_sqr. rewrite H3 H2 H1 -H7 H10. rewrite -ZModpRing.exprM => />.
+  congr. have ->: 2 * 2 ^ (i{hr} - 1) = 2^1 * 2 ^ (i{hr} - 1). rewrite expr1 //.
+  rewrite -exprD_nneg //. smt().
+  move => h II H8 [H9] [H10] [H11] [H12] H13. rewrite H12 -H11 H7 H13.
+  smt(op_it_sqr1_0).
+ qed.
 
 (** step 9 : invert **)
-lemma eq_h2_invert (z : zp) : 
-  hoare[MHop2.invert : z1' =  z ==> res = invert2 z].
+lemma eq_proc_op_invert (z : zp) :
+  hoare[CurveProcedures.invert : fs = z ==> res = op_invert2 z].
 proof.
   proc.
-  inline MHop2.sqr MHop2.mul.  wp.
-  ecall (eq_h2_it_sqr 4   t1). wp.
-  ecall (eq_h2_it_sqr 50  t2). wp.
-  ecall (eq_h2_it_sqr 100 t2). wp.
-  ecall (eq_h2_it_sqr 50  t1). wp.
-  ecall (eq_h2_it_sqr 10  t2). wp.
-  ecall (eq_h2_it_sqr 20  t2). wp.
-  ecall (eq_h2_it_sqr 10  t1). wp.
-  ecall (eq_h2_it_sqr 4   t2). wp.
+  inline CurveProcedures.sqr CurveProcedures.mul.  wp.
+  ecall (eq_proc_op_it_sqr 4   t1s). wp.
+  ecall (eq_proc_op_it_sqr 50  t2s). wp.
+  ecall (eq_proc_op_it_sqr 100 t2s). wp.
+  ecall (eq_proc_op_it_sqr 50  t1s). wp.
+  ecall (eq_proc_op_it_sqr 10  t2s). wp.
+  ecall (eq_proc_op_it_sqr 20  t2s). wp.
+  ecall (eq_proc_op_it_sqr 10  t1s). wp.
+  ecall (eq_proc_op_it_sqr 4   t2s). wp.
   skip. simplify.
-  move => &hr ?. 
+  move => &hr H.
   move=> ? ->. move=> ? ->. 
   move=> ? ->. move=> ? ->.
   move=> ? ->. move=> ? ->.
   move=> ? ->. move=> ? ->.
-  rewrite invert2E /sqr /= H /#.
+  rewrite op_invert2E /sqr /= H /#.
 qed.
 
-(** step 10 : encode point **)
-lemma eq_h2_encode_point (q : zp * zp) : 
-  hoare[MHop2.encode_point : x2 =  q.`1 /\ z2 = q.`2 ==> res = encodePoint1 q].
+
+equiv eq_proc_proc_invert:
+  CurveProcedures.invert_helper ~ CurveProcedures.invert:
+  fs{1} = fs{2} ==> res{1} = res{2}.
 proof.
-  proc. inline MHop2.mul. wp. sp.
-  ecall (eq_h2_invert z2).
+  proc => //=; inline CurveProcedures.sqr CurveProcedures.mul; wp.
+  call eq_sqr; wp. call eq_sqr; wp. call eq_sqr; wp.
+  call eq_sqr; wp. call eq_sqr; wp. call eq_sqr; wp.
+  call eq_sqr; wp. call eq_sqr; wp.
+  skip => />. smt().
+qed.
+
+
+(** step 10 : encode point **)
+lemma eq_proc_op_encode_point (q : zp * zp) :
+  hoare[CurveProcedures.encode_point : x2 =  q.`1 /\ z2 = q.`2 ==> res = op_encode_point q].
+proof.
+  proc. inline CurveProcedures.mul. wp. sp.
+  ecall (eq_proc_op_invert z2).
   skip. simplify.
-  move => &hr [?] [?] ? ?. move=> ->.
-  rewrite encodePoint1E /= H0 H1 //.
+  move => &hr [H] [H0] H1 H2 H3. 
+  rewrite op_encode_pointE.
+  auto => />. congr; congr; congr. rewrite -H1. apply H3.
 qed.
 
 (** step 11 : scalarmult **)
-lemma eq_h2_scalarmult (k u : W256.t) : 
-  hoare[MHop2.scalarmult : k' = k /\ u' = u ==> res = scalarmult k u].
+lemma eq_proc_op_scalarmult_internal (u: zp, k: W256.t) : 
+  hoare[CurveProcedures.scalarmult_internal : k.[0] = false  /\ k' = k /\ u'' = u ==> res = op_scalarmult_internal u k].
 proof.
-  rewrite -eq_scalarmult1.
-  proc. sp.
-  ecall (eq_h2_encode_point (x2,z2)).     simplify.
-  ecall (eq_h2_montgomery_ladder u'' k'). simplify.
-  ecall (eq_h2_decode_u_coordinate u').   simplify.
-  ecall (eq_h2_decode_scalar_25519 k').   simplify.
-  skip.
-  move => &hr [?] [?] [?] [?] [?] [?] ?.
-  move=> ? -> ? ->. split.
-    by rewrite /decodeScalar25519 /=.
-  move=> ? ? ? ? -> => /#.
+  proc; sp.
+  ecall (eq_proc_op_encode_point (x2, z2)). simplify.
+  ecall (eq_proc_op_montgomery_ladder u'' k'). simplify. skip.
+  move => &1 [H0] [H1] [H2] [H3] [H4] [H5] [H6] H7. split.
+  rewrite H6 => />.
+  move => H8 H9 H10 H11 H12. smt().
 qed.
+
+lemma eq_proc_op_scalarmult (k u : W256.t) :
+  hoare[CurveProcedures.scalarmult : k' = k /\ u' = u ==> res = spec_scalarmult k u].
+proof.
+  rewrite -eq_op_scalarmult.
+  proc.
+  pose dk := spec_decode_scalar_25519 k.
+  have kb0f  : (dk).[0] = false. (* k bit 0 false *)
+    rewrite /dk /spec_decode_scalar_25519 //.
+  ecall (eq_proc_op_scalarmult_internal u'' k').
+  ecall (eq_proc_op_decode_u_coordinate u').
+  ecall (eq_proc_op_decode_scalar k'). 
+  simplify. sp. skip.
+  move => &hr [H] [H0] H1 H2 H3 H4 H5. split.rewrite H3 H0. apply kb0f.
+  move=> H6 H7 ->. rewrite !op_encode_pointE. auto => />. congr. congr. congr. congr. congr.
+  rewrite H5 H3 H1 H0 => />.
+rewrite H5 H1 H3 H0 => />.
+ qed.
+
+lemma eq_proc_op_scalarmult_base (k : W256.t) :
+  hoare[CurveProcedures.scalarmult_base : k' = k ==> res = spec_scalarmult_base k].
+proof.
+  rewrite -eq_op_scalarmult_base.
+  proc.
+  pose dk := spec_decode_scalar_25519 k.
+  have kb0f  : (dk).[0] = false. (* k bit 0 false *)
+      rewrite /dk /spec_decode_scalar_25519 //.
+  ecall (eq_proc_op_scalarmult_internal u'' k').
+  ecall (eq_proc_op_decode_u_coordinate_base).
+  ecall (eq_proc_op_decode_scalar k').   simplify. sp. skip.
+  move => &hr [H] [H0] [H1] [H2] [H3] H4 H5 H6 H7 H8. split. rewrite H6 H4. apply kb0f.
+  move=> H9 H10 ->. rewrite /op_scalarmult_base  /op_scalarmult. auto => />.
+  rewrite !op_encode_pointE. progress. congr; congr; congr; congr. congr. congr.
+  rewrite H6 H4 => />. congr. congr. congr. rewrite H6 H4 => />.
+ qed.
